\documentclass[UTF8]{ctexart}

\usepackage{amsthm}
\usepackage{amsmath}
\usepackage{amssymb}
\usepackage{mathtools}
\usepackage{fancyhdr} 
\pagestyle{fancy}
\lhead{}
\chead{}
\rhead{}
\lfoot{}
\cfoot{}
\rfoot{\thepage}
\renewcommand{\headrulewidth}{0pt} 
\renewcommand{\footrulewidth}{0pt}

\title{最优化第四次作业}
\author{郭英明}
\date{2020/11/6}



\begin{document}
\maketitle
\section{}
\subsection{}
\textbf{1.To prove self-concordant function preserves properties under positive scaling $\alpha\geq0$, and sum}\\
Let
$$
  h(x)=\alpha f(x)\quad(\alpha\geq0)
$$
We know $f$ is self-concordant, then
$$
  |f^{'''}(x)|\leq2f^{''}(x)^{\frac{3}{2}}
$$
if $h$ is self-concordant, then
  $$|h^{'''}(x)|\leq2h^{''}(x)^{\frac{3}{2}}$$
  $$\alpha|f^{'''}(x)|\leq2\alpha^{\frac{3}{2}}f^{''}(x)^{\frac{3}{2}}$$
if $\alpha>0$,
  $$|f^{'''}(x)|\leq2\alpha^{\frac{1}{2}}f^{''}(x)^{\frac{3}{2}}$$
if $\alpha\geq1$, it satisfies\\
if $f(x_{i})\ (i \in [1,n])$ is self-concordant,then
  $$|f^{'''}(x_{i})|\leq2f^{''}(x_{i})^{\frac{3}{2}}\quad i\in[1,n]$$
  $$\sum\limits_{i=1}^{n}|f^{'''}(x_{i})|\leq2\sum\limits_{i=1}^{n}f^{''}(x_{i})^{\frac{3}{2}},\quad i\in(1,n)$$
for $h(x)=\sum\limits_{i=1}^{n}f(x_{i})$
if $h(x)$ is self-concordant, then
  $$|h^{'''}(x)|\leq2h^{''}(x)^{\frac{3}{2}}$$
  $$|\sum\limits_{i=1}^{n}f^{'''}(x_{i})|\leq2\sum\limits_{i=1}^{n}f^{''}(x_{i})^{\frac{3}{2}},\quad i\in[1,n]$$
Due to
  $$|\sum\limits_{i=1}^{n}f^{'''}(x_{i})|\leq\sum\limits_{i=1}^{n}|f^{'''}(x_{i})|,\quad i\in[1,n]$$
It satisfies\\

\subsection{}
\textbf{2.To prove self-concordant function preserves properties under composition with affine function}\\
Let
$$h(x)=f(ax+b)$$
we have
  $$h^{''}(x)=a^{2}f^{''}(ax+b)$$
  $$h^{'''}(x)=a^{3}f^{'''}(ax+b)$$
if $h$ is self-concordant, then
  $$|h^{'''}(x)|\leq2h^{''}(x)^{\frac{3}{2}}$$
  $$|a^{3}f^{'''}(ax+b)|\leq 2(a^{2}f^{''}(ax+b))^{\frac{3}{2}}$$
which (after dividing by $a^{3}$) is the self-concordant inequality for $f$\\

\subsection{}
\textbf{3.To prove if $g$ is convex with $dom\ g= R_{++}$ and $|g^{'''}(x)|\leq3g^{''}/x$, then $f(x)=-log(-g(x))-log(x)$ is self-concordant}\\
$$f^{''}(x)=\frac{x^{2}(g^{'}(x)^{2}-g(x)g^{''}(x))+g(x)^{2}}{x^{2}g(x)^{2}}$$
$$f^{'''}(x)=\frac{3g(x)g^{'}(x)g^{''}(x)-g(x)^{2}g^{'''}(x)-2g^{'}(x)^{3}}{g(x)^{3}}-\frac{2}{x^{3}}$$
According to  $g^{'''}(x)\leq3\frac{g^{''}(x)}{x}$
$$|f^{'''}(x)|\leq\frac{3g''(x)}{-xg(x)}+2(\frac{|g'(x)|}{-g(x)})^{3}+\frac{3g''(x)|g'(x)|}{g(x)^{2}}+\frac{2}{x^{3}}$$
if $f(x)$ is self-concordant, then it needs  to satisfies
$$f^{'''}(x)\leq2f^{''}(x)^{3/2}$$
So we can transfer the original problem to
$$\frac{\frac{3g''(x)}{-xg(x)}+2(\frac{|g'(x)|}{-g(x)})^{3}+\frac{3g''(x)|g'(x)|}{g(x)^{2}}+\frac{2}{x^{3}}}{2((\frac{g'(x)}{g(x)})^{2}-\frac{g''(x)}{g(x)}+\frac{1}{x^{2}})^{\frac{3}{2}}}\leq 1$$
We supposing
$$a=\frac{(-g''(x)/g(x))^{\frac{1}{2}}}{((\frac{g'(x)}{g(x)})^{2}-\frac{g''(x)}{g(x)}+\frac{1}{x^{2}})^{\frac{1}{2}}}$$
$$b=\frac{-\frac{|g'(x)|}{g(x)}}{((\frac{g'(x)}{g(x)})^{2}-\frac{g''(x)}{g(x)}+\frac{1}{x^{2}})^{\frac{1}{2}}}$$
$$c=\frac{\frac{1}{x}}{((\frac{g'(x)}{g(x)})^{2}-\frac{g''(x)}{g(x)}+\frac{1}{x^{2}})^{\frac{1}{2}}}$$
$$\{a,b,c>0\ |\ a^{2}+b^{2}+c^{2}=1\}$$
Then we just need to prove
$$\frac{3}{2}a^{2}c+b^{3}+\frac{3}{2}a^{2}b+c^{3}\leq1$$
$$\frac{3}{2}a^{2}c+b^{3}+\frac{3}{2}a^{2}b+c^{3}=\frac{1}{2}(b+c)(3-(b+c)^{2})\leq1$$
So $f(x)$ is self-concordant\\

\section{}
\subsection{}
\textbf{1.To prove $-\sum\limits_{i=1}^{m}log(b_{i}-a_{i}^{T}x)\ on\ \{x\ |\ a_{i}^{T}x<b_{i},\ i=1,2,\cdots,m\}$ is self-concordant}\\
let $$g(x)=-log(b-a^{T}x)$$
$$g^{''}(x)=\frac{(a^{T})^{2}}{(b-a^{T}x)^{2}}$$
$$g^{'''}=\frac{2(a^{T})^{3}}{(b-a^{T}x)^{3}}$$
$$\frac{g^{'''}(x)}{2g^{''}(x)^{3/2}}=1$$
$g(x)$ is self-concordant\\
According to function preserves self-concordant under sum\\
$f(x)=\sum\limits_{i=1}^{m}g(x)$ is self-concordant\\

\subsection{}
\textbf{2.To prove $f(X)=-log\ det(X)\ on\ S^{n}_{++}$ is self-concordant}\\
$$f^{''}(X)=-(X^{-2})^{T}$$
$$f^{'''}(X)=-2(X^{-3})^{T}$$
$$\frac{f^{'''}(X)}{2f^{''}(X)^{3/2}}=1$$
$f(X)$ is self-concordant\\

\subsection{}
\textbf{3.To prove $f(x,y)=-log(y^{2}-x^{T}x)\ on\ \{(x,y)\ |\ ||x||_{2}<y\}$ is self-concordant}\\
Limit the function to lines:$x=\hat x+tv,\ y= \hat y +tw$\\
Then we have
$$f( \hat x +tv, \hat y +tw)=-log(\hat y +tw) - log (\hat y +tw -\frac{(\hat x)^{T}\hat x +2t (\hat x)^{T}v+t^{2}v^{T}v}{\hat y +tw})$$
when $w=0$
$$f(t)=-log((\hat y)^{2}-(\hat x+tv)^{2})\quad dom f =\{ t \big| (\hat y)^{2}-(\hat x+tv) > 0\}$$
$$f(t)=-log(w^{2}(t-a)(t-b))=-log(w^{2})-log(t-a)-log(t-b)\quad (a,b\ are\ the\ solutions)$$
As $-log\ x$ is self-concordant and affine principles, $f(x,y)$ is self-concordant\\
when $w\neq0$, let $t=\frac{y-\hat y}{w}$\\
$$f=-log(\alpha+\beta y - \frac{\gamma}{y})-log(y)$$
$$\alpha=2\frac{\hat y v^{T}v}{w^{2}}-2\frac{(\hat x)^{T}v}{w}$$
$$\beta=1-\frac{v^{T}v}{w}$$
$$\gamma=(\hat x)^{T}(\hat x)-2\frac{\hat y (\hat x)^{T}v}{w}+\frac{(\hat y )^{2} v^{T}v}{w^{2}}$$
let $g(y)=-\alpha - \beta y +\frac{\gamma}{y} $,\\
then $$f(\hat x +tv, \hat y +tw)=-log(-g(y))-log(y)$$
$$g''(y)=\frac{2\gamma}{y^{3}}$$
$$g'''(y)=-\frac{6\gamma}{y^{4}}$$
$$ |g'''(y)| \leq \frac{3g''(y)}{y}\ and\ g(x)\ is \ convex$$
According to problem 3, $f(x,y)$ is self-concordant\\

\section{}
\subsection{}

\textbf{1.To rewrite $B^{+}=B+\frac{(y-Bs)(y-Bs)^{T}}{(y-Bs)^{T}s}$ as $C^{+}=C+\frac{(s-Cy)(s-Cy)^{T}}{(s-Cy)^{T}y}$}\\
According to Sherman-Morrison formula:
$$(A+uv{T})^{-1}=A^{-1}-\frac{A^{-1}uv^{T}A^{-1}}{1+v^{T}A^{-1}u}$$
$$C^{+}=C-\frac{C(y-Bs)(y-Bs)^{T}C}{1+(y-Bs)^{T}C(y-Bs)}$$
As $BC=I,\ (y-Bs)^{T}s=1$
$$C^{+}=C-\frac{(s-Cy)(s-Cy)^{T}}{(y-Bs)^{T}s+(y-Bs)^{T}(Cy-s)}$$
$$C^{+}=C+\frac{(s-Cy)(s-Cy)^{T}}{(s-Cy)^{T}y}$$

\subsection{}
\textbf{2.To rewrite $B^{+}=B-\frac{Bss^{T}B}{s^{T}Bs}+\frac{yy^{T}}{y^{T}s}$ as $C^{+}=(I-\frac{sy^{T}}{y^{T}s})C(I-\frac{ys^{T}}{y^{T}s})+\frac{ss^{T}}{y^{T}s}$}
According to Sherman-Morrison formula:
$$(A+\frac{uu^{t}}{t})^{-1}=A^{-1}-\frac{A^{-1}(uu^{T})A^{-1}}{t+u^{T}A^{-1}u}$$
$$(B+\frac{yy^{T}}{y^{T}s}-\frac{Bss^{T}B^{T}}{s^{T}Bs})^{-1}=(B+\frac{yy^{T}}{y^{T}s})^{-1}+\frac{(B+\frac{yy^{T}}{y^{T}s})^{-1}Bss^{T}B(B+\frac{yy^{T}}{y^{T}s})^{-1}}{s^{T}Bs-s^{T}B(B+\frac{yy^{T}}{y^{T}s})^{-1}Bs}$$
$$C^{+}=(B+\frac{yy^{T}}{y^{T}s})^{-1}+(B+\frac{yy^{T}}{y^{T}s})^{-1}\frac{Bss^{T}B}{s^{T}Bs-s^{T}B(B+\frac{yy^{T}}{y^{T}s})^{-1}Bs}(B+\frac{yy^{T}}{y^{T}s})^{-1}$$
$$C^{+}=C+\frac{ss^{T}y^{T}s}{(s^{T}y)^{2}}+\frac{ss^{T}yCy^{T}}{(s^{T}y)^{2}}-\frac{Cys^{T}}{s^{T}y}-\frac{sy^{T}C}{y^{T}s}$$
$$C^{+}=C(I-\frac{sy^{T}}{y^{T}s})-\frac{sy^{T}C}{s^{T}y}(I-\frac{sy^{T}}{s^{T}y})+\frac{ss^{T}}{s^{T}y}=(I-\frac{sy^{T}}{y^{T}s})C(I-\frac{ys^{T}}{y^{T}s})+\frac{ss^{T}}{y^{T}s}$$


\subsection{}
\textbf{3.We know $C^{+}=C-\frac{Cyy^{T}C}{y^{T}Cy}+\frac{ss^{T}}{y^{T}s}$, to prove $B^{+}=(I-\frac{ys^{T}}{y^{T}s})B(I-\frac{sy^{T}}{y^{T}s})+\frac{yy^{T}}{y^{T}s}$}\\
$$(C^{+})^{-1}=(C+\frac{ss^{T}}{y^{T}s})^{-1}+\frac{(C+\frac{ss^{T}}{y^{T}s})^{-1}Cyy^{T}C(C+\frac{ss^{T}}{y^{T}s})^{-1}}{y^{T}Cy+y^{T}C(C+(\frac{ss^{T}}{y^{T}s})^{-1}Cy}$$
$$(C^{+})^{-1}=C^{-1}+\frac{yy^{T}ys}{(s^{T})^{2}}+\frac{yy^{T}SC^{-1}S^{T}}{(s^{T}y)^{2}}-\frac{C^{-1}sy^{T}}{y^{T}s}-\frac{ys^{T}C^{-1}}{s^{T}y}$$
$$(C^{+})^{-1}=C^{-1}(I-\frac{sy^{T}}{y^{T}s})-\frac{ys^{T}C^{-1}}{s^{T}y}(I-\frac{ys^{T}}{s^{T}y})+\frac{yy^{T}}{s^{T}y}$$
$$B^{+}=(I-\frac{ys^{T}}{y^{T}S})B(I-\frac{sy^{T}}{y^{T}s})+\frac{yy^{T}}{y^{T}s}$$




\end{document}
